kore/src/theories/simple/InjectionTest2.v
@@ -22,11 +22,45 @@ Ltac autorewrite_set :=
     rewrite fmap_propset_singleton
   ).
 
+Ltac classicize :=
+  apply Classical_Prop.imply_to_or.
+Ltac app_ext_rewrite C :=
+lazymatch C with
+| context [propset_fa_union ?Cnew] =>
+    erewrite propset_fa_union_rewrite; [
+    |
+      intro;
+      match goal with
+      | |- ?G => app_ext_rewrite G
+      end;
+      unfold propset_fa_union;
+      try rewrite propset_double;
+      reflexivity
+    ]
+
+| context [app_ext ?sym _] =>
+  repeat (rewrite_app_ext; repeat rewrite fmap_propset_singleton);
+  autorewrite_set;
+  apply propset_top_eq;
+  repeat rewrite singleton_subseteq;
+  repeat rewrite singleton_eq;
+  simpl;
+  reflexivity
+end.
+Ltac app_ext_rewrite_all :=
+repeat match goal with
+| |- context [propset_fa_union ?C] =>
+    app_ext_rewrite (propset_fa_union C); unfold propset_fa_union at 1;
+    rewrite propset_double
+end.
+
 Ltac basic_simplify_krule :=
-  eval_helper2;
+  repeat eval_simplifier;
   simpl sort_inj;
-  repeat (rewrite_app_ext; try rewrite fmap_propset_singleton);
+  app_ext_rewrite_all;
+  repeat (rewrite_app_ext; repeat rewrite fmap_propset_singleton);
   autorewrite_set.
+
 Ltac simplify_krule :=
   basic_simplify_krule;
   apply propset_top_elem_of_2;
@@ -35,17 +69,6 @@ Ltac simplify_krule :=
   repeat rewrite elem_of_PropSet;
   repeat rewrite singleton_subseteq;
   repeat rewrite singleton_eq.
-
-
-Ltac abstract_var := 
-  match goal with
-    | [|- context [evar_valuation ?σ ?s]] =>
-      let x := fresh "var" in
-      let Hx := fresh "Hvar" in
-        remember (evar_valuation σ s) as x eqn:Hx (*;
-        clear Hx;
-        revert x *)
-    end.
 
 Module T.
 
@@ -338,7 +361,7 @@ Module T.
     (* Generate a goal for each axiom: *)
     unfold_elem_of; destruct_or?; destruct_ex?; subst; cbn.
     * by simplify_krule.
-(*    Step-by-step simplification would look like this:
+(* (*    Step-by-step simplification would look like this: *)
       rewrite eval_simpl.
       apply propset_top_elem_of_2;
       intro;
@@ -384,19 +407,16 @@ Module T.
       { remember (evar_valuation _ _) as l. clear.
         induction l. by simpl.
         simpl. by rewrite IHl. }
-    * simplify_krule. remember (fresh_evar _ _) as F.
-      simpl bevar_subst. cbn.
-      do 2 abstract_var.
+    * simplify_krule.
       destruct (klist_islist _) eqn:P; destruct b.
       2: by right.
-      left. intros []. subst var var0.
+      left. intros [].
       apply H. clear H.
       destruct (evar_valuation ρ "K"); simpl in *; try congruence.
       destruct c; simpl in *; try congruence.
       destruct x0; simpl in *; try congruence.
-      exists l. basic_simplify_krule.
-      apply elem_of_PropSet. apply singleton_subseteq.
-      rewrite decide_eq_same.
-      rewrite update_evar_val_diff_sort. congruence.
-      by rewrite H0.
+      exists l.
+      assumption.
   Qed.
+
+End T.
