kore/src/theories/simple/MInt.v
@@ -1,5 +1,5 @@
 From MatchingLogic Require Export stdpp_ext.
-From Kore Require Export Semantics.
+From Kore Require Export Semantics DVParsers.
 Import Signature.StringVariables.
 Import Kore.Syntax.Notations.
 
@@ -9,9 +9,6 @@ Open Scope kore_scope.
 Open Scope hlist_scope.
 Open Scope string_scope.
 
-(**
-   This is copied from the other file.
- *)
 Ltac autorewrite_set :=
   repeat (
     rewrite intersection_top_l_L +
@@ -25,10 +22,43 @@ Ltac autorewrite_set :=
     rewrite fmap_propset_singleton
   ).
 
+Ltac classicize :=
+  apply Classical_Prop.imply_to_or.
+Ltac app_ext_rewrite C :=
+lazymatch C with
+| context [propset_fa_union ?Cnew] =>
+    erewrite propset_fa_union_rewrite; [
+    |
+      intro;
+      match goal with
+      | |- ?G => app_ext_rewrite G
+      end;
+      unfold propset_fa_union;
+      try rewrite propset_double;
+      reflexivity
+    ]
+
+| context [app_ext ?sym _] =>
+  repeat (rewrite_app_ext; repeat rewrite fmap_propset_singleton);
+  autorewrite_set;
+  apply propset_top_eq;
+  repeat rewrite singleton_subseteq;
+  repeat rewrite singleton_eq;
+  simpl;
+  reflexivity
+end.
+Ltac app_ext_rewrite_all :=
+repeat match goal with
+| |- context [propset_fa_union ?C] =>
+    app_ext_rewrite (propset_fa_union C); unfold propset_fa_union at 1;
+    rewrite propset_double
+end.
+
 Ltac basic_simplify_krule :=
-  eval_helper2;
+  repeat eval_simplifier;
   simpl sort_inj;
-  repeat (rewrite_app_ext; try rewrite fmap_propset_singleton);
+  app_ext_rewrite_all;
+  repeat (rewrite_app_ext; repeat rewrite fmap_propset_singleton);
   autorewrite_set.
 
 Ltac simplify_krule :=
@@ -220,7 +250,8 @@ Module NonRecursive.
            end
     )
     _
-    (λ s s' H, match H with end).
+    (λ s s' H, match H with end)
+    (fun _ => None_parser).
 
   Definition test : @Theory MintSignature := PropSet (λ pat,
     (* --x = x *)
